\documentclass[11pt]{article}
\usepackage{amsmath,amssymb,amsthm,mathrsfs,graphicx}

\newcommand{\N}{\mathbb{N}}

\title{MATH 3283W Written Project}
\author{Amolak Singh}
\date{Spring 2016}

\begin{document}

\maketitle

\subsubsection*{Definition of Mathematical Induction.}

Let $P(n)$ be a statement $\mbox{ for all } n\in \N.$  $P(n)$ is true if $P(1)$ is true, and $P(k)$ implies $P(k+1) \mbox{ for each } k\in \N.$ We will use induction to prove the statement below.

\subsubsection*{Section 3.4 \# 4.}
Prove that $1^{3} + 2^{3} + \cdots + n^{3} = \frac{n^{2}(n+1)^{2}}{4}, \mbox{ for all } n\in \N.$ \\

Let $P(n)$ be the statement $1^{3} + 1^{3} + \cdots + n^{3} = \frac{n^{2}(n+1)^{2}}{4}, \mbox{ for all } n\in \N.$\\

First, we will verify that $P(1)$ is true. 
On the right hand side, $P(1) = 1^{3} = 1.$ 
On the left hand side, $P(1) = \frac{1^{2}*(1+1)^{2}}{4} = \frac{1*4}{4} = 1.$ 
Thus, $P(1)$ is true. \\

Now, we will show that $P(k+1)$ follows from $P(k)$. 
Suppose $P(k)$ is true $\mbox{ for all } k = n\in \mathbb{N}.$
We have the following equalities:

\begin{align*}
&= \frac{k^{2}(k+1)^{2}}{4} + (k+1)^{3}\\
&= \frac{k^{2}(k+1)^{2}+4(k+1)^{3}}{4}\\
&= \frac{k^{4}+6k^{3}+13k^{2}+4}{4} \\
&= \frac{(k+1)^{2}(k+2)^{2}}{4} \\
&= \frac{(k+1)^{2}(k+1+1)^{2}}{4}.
\end{align*}
\\  

Since $P(1)$ is true, and $P(k)$ implies $P(k+1)$, $P(n)$ is true for all natural numbers by mathematical induction.

\subsubsection*{Discussion.}

It is easy to see that {(3.4 \#5)} follows from this proof by the following equalities:
$$1^{3} + 1^{3} + \cdots + n^{3} = \frac{n^{2}(n+1)^{2}}{4} = \left(\frac{n(n+1)}{2}\right)^{2} = (1^{2} + 2^{2} + \cdots + n^{2})^{2}.$$ \\

We can also see that the sum of $n^{k}$ natural numbers always has a summation formula with a leading term of the form $n^{k+1}$. For example, the summation formula for naturals has a leading $n^{2}$ term, the summation for squares has a leading $n^{3}$ term, and the summation for cubes has a leading $n^{4}$ term. See the formulas below:

$$1 + 2 + \cdots + n = \frac{(n+1)(n+2)}{2}$$
$$1^{2} + 2^{2} + \cdots + n^{2} = \frac{n(n+1)(2n+1)}{6}$$
$$1^{3} + 2^{3} + \cdots + n^{3} = \frac{n^{2}(n+1)^{2}}{4}.$$

\end{document}
